# Problem

Solve the recurrence ![T(n)=2T(n/2)+n-1](http://latex.codecogs.com/gif.latex?T%28n%29%3D2T%28%5Cfrac%7Bn%7D%7B2%7D%29%2Bn-1) where ![n=2^k](http://latex.codecogs.com/gif.latex?n%3D2%5Ek) is assumed; assume that ![T(n)](http://latex.codecogs.com/gif.latex?T%28n%29) is constant if ![n<=2](http://latex.codecogs.com/gif.latex?n%5Cleqq2).

# Solution

![T(n)=(n-1)+2T(n/2)](http://latex.codecogs.com/gif.latex?T%28n%29%3D%28n-1%29%2B2T%28%5Cfrac%7Bn%7D%7B2%7D%29)

![=(n-1)+2((n/2-1)+2T(n/4))](http://latex.codecogs.com/gif.latex?%3D%28n-1%29%2B2%28%28%5Cfrac%7Bn%7D%7B2%7D-1%29%2B2T%28%5Cfrac%7Bn%7D%7B4%7D%29%29)

![=(n-1)+(n-2)+4T(n/4)](http://latex.codecogs.com/gif.latex?%3D%28n-1%29%2B%28n-2%29%2B4T%28%5Cfrac%7Bn%7D%7B4%7D%29)

![=(n-1)+(n-2)+4((n/4-1)+2T(n/8))](http://latex.codecogs.com/gif.latex?%3D%28n-1%29%2B%28n-2%29%2B4%28%28%5Cfrac%7Bn%7D%7B4%7D-1%29%2B2T%28%5Cfrac%7Bn%7D%7B8%7D%29%29)

![=(n-1)+(n-2)+(n-4)+8T(n/8)](http://latex.codecogs.com/gif.latex?%3D%28n-1%29%2B%28n-2%29%2B%28n-4%29%2B8T%28%5Cfrac%7Bn%7D%7B8%7D%29)

---

![=(n-1)+(n-2)+(n-4)+…+(n-2^(k-2))+2^(k-1)T(2)](http://latex.codecogs.com/gif.latex?%3D%28n-1%29%2B%28n-2%29%2B%28n-4%29%2B...%2B%28n-2%5E%7Bk-2%7D%29%2B2%5E%7Bk-1%7DT%282%29)

---

![=(k-1)n–(2^(k-1)-1)+2^(k-1)T(2)](http://latex.codecogs.com/gif.latex?%3D%28k-1%29n-%282%5E%7Bk-1%7D-1%29%2B2%5E%7Bk-1%7DT%282%29)

![=(log(n-1))n–n/2+n/2T(2)+1](http://latex.codecogs.com/gif.latex?%3D%28log_2n-1%29n-%5Cfrac%7Bn%7D%7B2%7D%2B%5Cfrac%7Bn%7D%7B2%7DT%282%29%2B1)

let T(2) be a constant C.

![=nlog_2n+(c-3)n/2+1](http://latex.codecogs.com/gif.latex?%3Dnlog_2n%2B%5Cfrac%7B%28c-3%29n%7D%7B2%7D%2B1)
